formal-proofs/theories/lib/interruptible_semaphore/async_immediate.v
@@ -12,18 +12,18 @@ Definition newSemaphore: val :=
   λ: "n", (ref "n", newThreadQueue array_interface #()).
 
 Definition acquireSemaphore: val :=
-  rec: "loop" "sem" :=
-    let: "availablePermits" := Fst ("sem") in
-    let: "e" := Fst (Snd ("sem")) in
-    let: "p" := FAA "availablePermits" #(-1) in
-    if: #0 < "p" then fillThreadQueueFuture #()
-    else match: suspend array_interface "e" with
-             NONE => "loop" "sem"
-           | SOME "v" => "v"
-         end.
+  λ: "sem",
+  let: "availablePermits" := Fst ("sem") in
+  let: "e" := Fst (Snd ("sem")) in
+  let: "p" := FAA "availablePermits" #(-1) in
+  if: #0 < "p" then fillThreadQueueFuture #()
+  else match: suspend array_interface "e" with
+           InjR "v" => "v"
+         | InjL "x" => "undefined"
+       end.
 
 Definition semaphoreResume: val :=
-  λ: "d", resume array_interface #(Z.of_nat 300) #true #true #true "d"
+  λ: "d", resume array_interface #(Z.of_nat 300) #false #false #false "d"
                  (λ: <>, #()) #().
 
 Definition releaseSemaphore: val :=
@@ -41,7 +41,7 @@ Definition cancelSemaphoreFuture : val :=
   let: "availablePermits" := Fst ("sem") in
   let: "d" := Snd (Snd ("sem")) in
   tryCancelThreadQueueFuture' array_interface
-                              #false #(Z.of_nat 300) #true #true
+                              #true #(Z.of_nat 300) #false #false
                               "d" (λ: <>, FAA "availablePermits" #1 < #0)
                               (λ: <>, #()) (λ: <>, releaseSemaphore "sem") "f".
 
@@ -74,7 +74,7 @@ Variable array_interface: infiniteArrayInterface.
 Variable array_spec: infiniteArraySpec _ array_interface.
 
 Let tqParams R :=
-  @ThreadQueueParameters Σ false True R True (fun v => ⌜#v = #()⌝)%I True.
+  @ThreadQueueParameters Σ true True R False (fun v => ⌜#v = #()⌝)%I False.
 
 Let isThreadQueue R := is_thread_queue NTq NFuture (tqParams R) _ array_spec.
 
@@ -102,14 +102,14 @@ Qed.
 
 Lemma resumeSemaphore_spec R maxWait (wait: bool) γa γtq γe γd e d:
   {{{ isThreadQueue R γa γtq γe γd e d ∗ awakening_permit γtq }}}
-    resume array_interface #(Z.of_nat maxWait) #true #true #wait d (λ: <>, #())%V #()
+    resume array_interface #(Z.of_nat maxWait) #false #false #wait d (λ: <>, #())%V #()
   {{{ (r: bool), RET #r; if r then True else R }}}.
 Proof.
   iIntros (Φ) "[#HTq HAwak] HΦ".
   iApply (resume_spec with "[] [HAwak]").
   5: { by iFrame "HTq HAwak". }
   by solve_ndisj. done. done.
-  { simpl. iIntros (Ψ) "!> _ HΨ". wp_pures. by iApply "HΨ". }
+  { simpl. iIntros (Ψ) "!> [% _] HΨ". done. }
   iIntros "!>" (r) "Hr". iApply "HΦ". simpl. destruct r; first done.
   by iDestruct "Hr" as "(_ & $ & _)".
 Qed.
@@ -154,7 +154,7 @@ Theorem acquireSemaphore_spec R γa γtq γe γd s:
   {{{ γf v, RET v; is_semaphore_future R γtq γa γf v ∗
                    thread_queue_future_cancellation_permit γf }}}.
 Proof.
-  iIntros (Φ) "#HIsSem HΦ". wp_lam. iLöb as "IH".
+  iIntros (Φ) "#HIsSem HΦ". wp_lam.
   iDestruct "HIsSem" as (e d p ->) "[HInv HTq]". wp_pures. wp_bind (FAA _ _).
   iInv "HInv" as (availablePermits) "[HRs HOpen]" "HClose".
   iDestruct "HOpen" as (enqueuedThreads) "(HState & Hp & >HPures)".
@@ -184,10 +184,10 @@ Proof.
       by replace (availablePermits - enqueuedThreads + -1)%Z with
           (availablePermits - S enqueuedThreads)%Z by lia. }
     iModIntro. wp_pures. rewrite bool_decide_false; last lia. wp_pures.
-    wp_apply (suspend_spec with "[$]")=> /=. iIntros (v) "[[-> _]|Hv]".
-    + wp_pures. wp_lam. iApply ("IH" with "HΦ").
-    + iDestruct "Hv" as (γf v') "(-> & HFuture & HCancPermit)". wp_pures.
-      iApply "HΦ". iFrame.
+    wp_apply (suspend_spec with "[$]")=> /=. iIntros (v) "[(_ & _ & %)|Hv]".
+    done.
+    iDestruct "Hv" as (γf v') "(-> & HFuture & HCancPermit)". wp_pures.
+    iApply "HΦ". iFrame.
 Qed.
 
 Theorem cancelSemaphoreFuture_spec R γa γtq γe γd s γf f:
@@ -211,59 +211,19 @@ Proof.
   iDestruct "Hr" as "[#HFutureCancelled Hr]". iFrame "HFutureCancelled".
   rewrite /is_semaphore_future /is_thread_queue_future.
   iDestruct "Hr" as (i f' s ->) "Hr"=> /=.
-  iDestruct "Hr" as "(#H↦~ & #HTh & HToken)". iIntros "!> HΦ !>". wp_pures.
-  wp_lam. wp_pures. wp_apply derefCellPointer_spec.
+  iDestruct "Hr" as "(#H↦~ & #HTh & #HInhabited & HCancHandle)".
+  iIntros "!> HΦ !>". wp_pures. wp_apply derefCellPointer_spec.
   by iDestruct "HTq" as "(_ & $ & _)". iIntros (ℓ) "#H↦". wp_pures.
-  wp_bind (FAA _ _).
-  iInv "HInv" as (availablePermits) "[HRs HOpen]" "HClose".
-  iDestruct "HOpen" as (enqueuedThreads) "(>HState & Hp & >HPures)".
-  iDestruct "HPures" as %HPures.
-  iMod (register_cancellation with "HTq HToken HState")
-       as "[HCancToken HState]"; first by solve_ndisj.
-  destruct (decide (availablePermits - enqueuedThreads < 0)%Z) as [HLt|HGe].
-  - assert (availablePermits = 0) as -> by lia.
-    destruct enqueuedThreads as [|enqueuedThreads']=>/=; first lia.
-    iDestruct "HState" as "(HState & HCancHandle & #HInhabited)".
-    wp_faa.
-    iMod ("HClose" with "[-HΦ HCancToken HCancHandle]") as "_".
-    { iExists 0. iSplitR; simpl; first done. iExists enqueuedThreads'.
-      rewrite Nat.sub_0_r. iFrame "HState". iSplitL; last by iLeft.
-      by replace (0%nat - S enqueuedThreads' + 1)%Z
-        with (0%nat - enqueuedThreads')%Z by lia. }
-    iModIntro. wp_pures. wp_bind (getAndSet.getAndSet _ _).
-    awp_apply (markCancelled_spec with "HTq HInhabited H↦ HCancToken HTh")
-              without "HΦ HCancHandle".
-    iAaccIntro with "[//]"; first done. iIntros (v) "Hv"=>/=.
-    iIntros "!> [HΦ HCancHandle]". wp_pures.
-    iAssert (▷ cell_cancellation_handle _ _ _ _ _ _)%I
-            with "[HCancHandle]" as "HCancHandle"; first done.
-    awp_apply (cancelCell_spec with "[] H↦~") without "Hv HΦ".
-    by iDestruct "HTq" as "(_ & $ & _)".
-    iAaccIntro with "HCancHandle". by iIntros "$".
-    iIntros "#HCancelled !> [Hv HΦ]". wp_pures.
-    iDestruct "Hv" as "[[-> _]|Hv]"; first by wp_pures.
-    iDestruct "Hv" as (x ->) "(#HInhabited' & HAwak & %)"; simplify_eq.
-    wp_pures. wp_apply (resumeSemaphore_spec with "[$]").
-    iIntros (r) "Hr". destruct r; wp_pures; first done.
-    wp_apply (releaseSemaphore_spec with "[Hr]").
-    { iSplitR; last by iApply "Hr". iExists _, _, _.
-      iSplitR; first done. iFrame "HInv HTq". }
-    iIntros "_". by wp_pures.
-  - rewrite bool_decide_true; last lia. assert (enqueuedThreads = 0) as -> by lia.
-    simpl. iDestruct "HState" as "(HState & HR & #HInhabited)".
-    wp_faa.
-    iMod ("HClose" with "[-HΦ HCancToken]") as "_".
-    { iExists (S availablePermits). iFrame "HR HRs". iExists 0.
-      iFrame "HState". iSplitL; last by iRight.
-      by replace (availablePermits - 0%nat + 1)%Z
-        with (S availablePermits - 0%nat)%Z by lia. }
-    iModIntro. wp_pures. rewrite bool_decide_false; last lia. wp_pures.
-    wp_bind (getAndSet.getAndSet _ _).
-    awp_apply (markRefused_spec with "HTq HInhabited H↦ HCancToken HTh [//]")
-              without "HΦ".
-    iAaccIntro with "[//]"; first done. iIntros (v) "Hv"=>/=.
-    iIntros "!> HΦ". iDestruct "Hv" as "[[-> _]|Hv]"; first by wp_pures.
-    iDestruct "Hv" as (? ->) "[_ >%]". simplify_eq. by wp_pures.
+  wp_bind (getAndSet.getAndSet _ _).
+  awp_apply (markCancelled_immediate_spec with "HTq HInhabited H↦")
+            without "HCancHandle HΦ".
+  iAaccIntro with "[//]". done. iIntros (?) "_ !> [HCancHandle HΦ]". wp_pures.
+  iAssert (▷ cell_cancellation_handle _ _ _ _ _ _)%I
+          with "[HCancHandle]" as "HCancHandle"; first done.
+  awp_apply (cancelCell_spec with "[] H↦~") without "HΦ".
+  by iDestruct "HTq" as "(_ & $ & _)".
+  iAaccIntro with "HCancHandle". by iIntros "$". iIntros "#HCancelled !> HΦ".
+  by wp_pures.
 Qed.
 
 End proof.
